Organización en carpetas

Turing Reducciones/Clique/POCToPC.dfy
@@ -1,16 +1,6 @@
 include "../../Especificaciones/Clique/CliqueOpt.dfy"
 include "../../Especificaciones/Clique/CliqueProperties.dfy"
-/*
-ghost predicate invariantLoop(
-  graph : Graph, okg : nat,
-  vertex : set<Node>,//remaining vertex
-  I : set<Node>, //up to now vertex cover
-  g : Graph, kg : nat//current graph
-)
-{ true }
-*/
-
-ghost predicate containedInAllSolutions()
+include "POCToPCAux.dfy"
 
 ghost predicate invariantLoop(
   graph : Graph, okg : nat,
@@ -23,32 +13,25 @@ requires isValidGraph(graph)
   //g is a valid subgraph of graph
   isValidGraph(g) &&
   isSubGraph(g, graph) &&
-  okg >= 1 &&
-  kg == okg &&
   //g has at leat okg vertices
   |g.0| >= okg &&
-  //while g has more than okg vertices, vertex is not empty
-  (|g.0| > okg ==> vertex != {}) &&
-  //the partial solution is subset of the vertices in g
-  I <= g.0 &&
-  //vertices that have not been analyzed are a subset of the vertices in g
-  vertex <= g.0 &&
-  //all vertices in the partial solution have been analyzed
+  //all vertices in the partial solution have been analyzed and are thus not in vertex
   I == g.0 - vertex &&
-  //TODO expresar esto de una mejor manera
-  (forall i: Node | i in I :: (forall G: Graph | isValidGraph(G) && isSubGraph(G, g) && optimalValueClique(G, kg) :: (forall S: set<Node> | S <= G.0 && optimalClique(G, S) :: i in S)))  &&
-  optimalValueClique(g, okg) && 
   //I is a prtial solution
-  (exists S: set<Node> :: S <= g.0 && optimalClique(graph, S) && I <= S) 
+  (forall i: Node | i in I :: (forall G: Graph | isValidGraph(G) && isSubGraph(G, g) && optimalValueClique(G, kg) :: (forall S: set<Node> | S <= G.0 && optimalClique(G, S) :: i in S)))  &&
+  optimalValueClique(g, okg)  
 
-  //g.1 +  (set edge:Edge, node:Node | edge in graph.1 && node in I && node in edge :: edge) == graph.1 &&
-
-  //At the end kg = 0 and |I| = okg, so I is optimal
-  //kg >= 0 && optimalValueVertexCover(g,kg) &&
-  //kg + |I| == okg //&&
-
-  //(forall u, O | u in g.0 && u !in vertex &&  I <= O <= graph.0 && isClique(graph, O) && |O| == okg :: u !in O) &&
-  //exists V : set<Node> :: V <= g.0 && optimalClique(graph, V) //&& optimalVertexCover(graph, I + V))
+  //The following invariants, although true, are not needed for the method to verify, but they can be useful to better understande the code
+  //g contains an optimal clique for graph
+  //kg == okg 
+  //while g has more than okg vertices, vertex is not empty
+  //(|g.0| > okg ==> vertex != {}) 
+  //the partial solution is subset of the vertices in g
+  //I <= g.0 
+  //vertices that have not been analyzed are a subset of the vertices in g
+  //vertex <= g.0 
+  //I con be extended to form an optimal clique for graph
+  //(exists S: set<Node> :: S <= g.0 && optimalClique(graph, S) && I <= S)
 }
 
 
@@ -63,61 +46,56 @@ method mOptimalClique (graph:Graph) returns (I:set<Node>)
   requires isValidGraph(graph)
   ensures optimalClique(graph, I)
 {
-  if graph.0 == {} { I := {}; }
-  else {
-    I := {};
-    //this is the initial set of vertex
-    //used to traverse the graph vertices
-    var vertex := graph.0; 
-    //Optimal Clique value for graph
-    var okg :=  moptimalValueClique(graph);
-    UpperBoundClique(graph);
-    assert okg <= |graph.0|; 
-    //Current graph, it contains nodes that have not been analyzed and nodes which have been analyzed to belong to an optimal Clique for graph
-    var g := graph; 
-    //Optimal Clique value for the current graph
-    var kg := moptimalValueClique(g);
+  I := {};
+  //this is the initial set of vertex
+  //used to traverse the graph vertices
+  var vertex := graph.0; 
+  //Optimal Clique value for graph
+  var okg :=  moptimalValueClique(graph);
+  //Current graph, it contains nodes that have not been analyzed and nodes which have been analyzed to belong to an optimal Clique for graph
+  var g := graph; 
+  //Optimal Clique value for the current graph
+  var kg := moptimalValueClique(g);
 
-    CliqueTranslation(g, kg);
-    nonEmptyClique(g);
+  //A clique for graph cannot contain more than |graph.0| vertices
+  UpperBoundClique(graph);
+  //If kg is the optimal value of a clique for g, there is some clique with that cardinality and no cliques with a greater cardinality
+  CliqueTranslation(g, kg);
 
-    //stop when g.0 == I
-    while (|I| < okg)
-      decreases vertex
-      invariant invariantLoop(graph,okg,vertex,I,g,kg)
-    {  
-      //UpperBoundClique(graph);
-      var v: Node := pick(vertex);
-      //Remove vertex v
-      var g' := removeVertex(g, v); 
-      validSubgraph(g,v,g');
-      var kg': nat := moptimalValueClique(g');
+  //stop when g.0 == I
+  while (|I| < okg)
+    decreases vertex
+    invariant invariantLoop(graph,okg,vertex,I,g,kg)
+  {  
+    var v: Node := pick(vertex);
+    //Remove vertex v
+    var g' := removeVertex(g, v); 
+    validSubgraph(g,v,g');
+    //Calculate the optimal value of a clique for the new graph
+    var kg': nat := moptimalValueClique(g');
 
-      //Only two options are possible
-      assert kg' == kg || kg == kg' + 1 by { ovCliqueRemoveVertex(g, g', v, kg, kg'); } 
-      if kg == kg' + 1 
-      { 
-        //any optimal clique for g must include v
-        isPartialSolutionWith2(g, g', v, kg, kg');
-        isPartialSolutionWith(g, g', v, kg, kg', I);
-        I := I + {v};
-        
-      }
-      //there exists an optimal clique that does not contain v
-      else { //kg == kg'
-        ghost var S: set<Node> :| S <= g'.0 && optimalClique(g', S);
-        CliqueInSubgraph(graph, g', kg, S);
-        isPartialSolutionWithout(g, g', v, kg, kg', I);
-        g := g';  
-        //TODO must prove it does not belong to some partial solution
-      }
-      vertex := vertex - {v};
-      assert exists S: set<Node> :: S <= g.0 && optimalClique(graph, S) && I <= S;
-      ghost var S: set<Node> :| S <= g.0 && optimalClique(graph, S) && I <= S;
-      cardinalityLemma3(S, g.0);
-      assert |g.0| >= |S|;
-      CliqueTranslation(g, kg);
+    //Only two options are possible, either the optimal value stays the same or it is one less than it was
+    assert kg' == kg || kg == kg' + 1 by { ovCliqueRemoveVertex(g, g', v, kg, kg'); } 
+    if kg == kg' + 1 
+    { 
+      //Any optimal clique for g must include v
+      isPartialSolutionWith2(g, g', v, kg, kg');
+      isPartialSolutionWith(g, g', v, kg, kg', I);
+      //v is included in our partial solution and stays in g
+      I := I + {v};
+      
     }
-    cardinalityLemma2();
+    else { //kg == kg'
+      //There exists an optimal clique that does not contain v
+      isPartialSolutionWithout(g, g', v, kg, kg', I);
+      //Since there is an optimal clique in g', we can remove v from the graph while maintaining that g contains an optimal clique
+      g := g';  
+    }
+    //vertex v has already been analyzed
+    vertex := vertex - {v};
+    assert exists S: set<Node> :: S <= g.0 && optimalClique(graph, S) && I <= S;
+    ghost var S: set<Node> :| S <= g.0 && optimalClique(graph, S) && I <= S;
+    //An optimal clique does not contain more than |g.0| vertices 
+    cardinalityLemma3(S, g.0);
   }
 }
