Especificaciones/Clique/CliqueProperties.dfy
@@ -50,44 +50,6 @@ lemma alwaysAnOptimalClique(g: Graph)
     assert optimalClique(g, S);
 }
 
-lemma nonEmptySetClique(g: Graph, k: nat)
-    requires isValidGraph(g)
-    requires g.0 != {}
-    requires optimalValueClique(g, k)
-      
-{ }
-
-lemma ovCliqueRemoveVertex(g: Graph, g': Graph, v: Node, kg: nat, kg': nat)
-    requires isValidGraph(g)
-    requires g' == removeVertex(g, v)
-    requires isSubGraph(g', g)
-    requires optimalValueClique(g, kg)
-    requires optimalValueClique(g', kg')
-    ensures kg' == kg || kg == kg' + 1
-{
-    if kg' > kg {
-        ghost var I: set<Node> :| I <= g'.0 && isClique(g', I) && |I| >= kg';
-        assert CliqueDecissionProblem(g, |I|);
-        assert false;
-    }
-    assert kg >= kg';
-    CliqueTranslation(g, kg);
-    //No entiendo por qué no es capaz de sacar cosas que están en la definición de optimalClique
-    ghost var I: set<Node> :| (optimalClique(g, I) && |I| == kg && I <= g.0 && isClique(g, I));
-    assert isClique(g, I);
-    assert v in I || v !in I;
-    if v !in I {
-        assert optimalValueClique(g', |I|);
-    }
-    else{
-        if exists I': set<Node> :: isClique(g', I') && |I'| == kg {}
-        else{
-            ghost var I': set<Node> := I - {v};
-            CliqueTranslation2(g', I');
-        }
-    } 
-}
-
 lemma CliqueTranslation(g: Graph, k: nat)
     requires isValidGraph(g)
     requires optimalValueClique(g, k)
@@ -114,6 +76,7 @@ lemma CliqueTranslation2(g: Graph, I: set<Node>)
     ensures optimalValueClique(g, |I|)
 { }
 
+//Generalization of CliqueTranslation2
 lemma CliqueTranslation2Gen(g: Graph)
     requires isValidGraph(g)
     ensures forall I: set<Node> | optimalClique(g, I) :: optimalValueClique(g, |I|)
@@ -126,20 +89,21 @@ lemma CliqueTranslation2Gen(g: Graph)
     }
 }
 
+//Generalization of CliqueTranslation3
+lemma CliqueTranslation3Gen(g: Graph, k: nat)
+    requires isValidGraph(g)
+    requires optimalValueClique(g, k)
+    ensures forall I: set<Node> | |I| == k && isClique(g, I) :: optimalClique(g, I)
+{ 
+    CliqueTranslation(g, k);
+}
+
 lemma CliqueTranslation3(g: Graph, k: nat, I: set<Node>)
     requires isValidGraph(g)
     requires optimalValueClique(g, k)
     requires k == |I|
     requires isClique(g, I)
     ensures optimalClique(g, I)
-{ 
-    CliqueTranslation(g, k);
-}
-
-lemma CliqueTranslation3Gen(g: Graph, k: nat)
-    requires isValidGraph(g)
-    requires optimalValueClique(g, k)
-    ensures forall I: set<Node> | |I| == k && isClique(g, I) :: optimalClique(g, I)
 { 
     CliqueTranslation(g, k);
 }
@@ -154,102 +118,4 @@ lemma CliqueInSubgraph(g: Graph, g': Graph, k: nat, S: set<Node>)
     ensures optimalClique(g, S)
 { 
     CliqueTranslation(g, k);
-}
-
-lemma isPartialSolutionWith1(g: Graph, g': Graph, v: Node, kg: nat, kg': nat)
-    requires isValidGraph(g)
-    requires isValidGraph(g')
-    requires g' == removeVertex(g, v)
-    //requires isSubGraph(g', g)
-    requires optimalValueClique(g, kg)
-    requires optimalValueClique(g', kg')
-    requires kg' < kg
-    ensures forall S: set<Node> | S <= g.0 && optimalClique(g, S) :: v in S
-{
-    //all optimal cliques in g must contain v
-    assert (forall A: set<Node> | optimalClique(g, A) :: v in A) by {
-        if exists A: set<Node> :: optimalClique(g, A) && v !in A
-        {
-            var A: set<Node> :| optimalClique(g, A) && v !in A;
-            assert isClique(g', A);
-            assert optimalValueClique(g', |A|);
-            assert |A| > kg';
-            assert false;
-        }
-    }
-}
-
-lemma isPartialSolutionWith2(g: Graph, g': Graph, v: Node, kg: nat, kg': nat)
-    requires isValidGraph(g)
-    requires isValidGraph(g')
-    requires g' == removeVertex(g, v)
-    requires optimalValueClique(g, kg)
-    requires optimalValueClique(g', kg')
-    requires kg' + 1 == kg
-    ensures forall G: Graph | isValidGraph(G) && isSubGraph(G, g) && optimalValueClique(G, kg) :: (forall S: set<Node> | S <= G.0 && optimalClique(G, S) :: v in S)
-{
-    //if there exists a subgraph whose optimal clique does not include v
-    if exists G: Graph :: isValidGraph(G) && isSubGraph(G, g) && optimalValueClique(G, kg) && (exists S: set<Node> :: S <= G.0 && optimalClique(G, S) && v !in S)
-    {
-        //instantiate the graph
-        var G: Graph :| isValidGraph(G) && isSubGraph(G, g) && optimalValueClique(G, kg) && (exists S: set<Node> :: S <= G.0 && optimalClique(G, S) && v !in S);
-        //instantiate the clique
-        var S: set<Node> :| S <= G.0 && optimalClique(G, S) && v !in S; 
-        //that clique must actually contain v, since it would be an optimal clique in g
-        CliqueTranslation2(G, S);
-        assert |S| == kg;
-        CliqueInSubgraph(g, G, |S|, S);
-        assert optimalClique(g, S);
-        isPartialSolutionWith1(g, g', v, kg, kg');
-    }
-}
-
-lemma isPartialSolutionWith(g: Graph, g': Graph, v: Node, kg: nat, kg': nat, I: set<Node>)
-    decreases I
-    requires isValidGraph(g)
-    requires isValidGraph(g')
-    requires g' == removeVertex(g, v)
-    requires optimalValueClique(g, kg)
-    requires optimalValueClique(g', kg')
-    requires kg' + 1 == kg
-    requires I <= g.0
-    requires |I| <= kg
-    requires forall i: Node | i in I :: (forall G: Graph | isValidGraph(G) && isSubGraph(G, g) && optimalValueClique(G, kg) :: (forall S: set<Node> | S <= G.0 && optimalClique(G, S) :: i in S));
-    ensures exists S: set<Node> :: S <= g.0 && I <= S && optimalClique(g, S) && v in S
-{
-    //all optimal cliques in g must contain v
-    assert (forall A: set<Node> | optimalClique(g, A) :: v in A) by {
-        if exists A: set<Node> :: optimalClique(g, A) && v !in A
-        {
-            var A: set<Node> :| optimalClique(g, A) && v !in A;
-            assert isClique(g', A);
-            assert optimalValueClique(g', |A|);
-            assert |A| > kg';
-            assert false;
-        }
-    }
-    alwaysAnOptimalClique(g);
-    assert exists S: set<Node> :: S <= g.0 && optimalClique(g, S) && v in S;
-    var S: set<Node> :| S <= g.0 && optimalClique(g, S) && v in S; 
-    assert forall i: Node | i in I :: i in S; 
-}
-
-
-lemma isPartialSolutionWithout(g: Graph, g': Graph, v: Node, kg: nat, kg': nat, I: set<Node>)
-    requires isValidGraph(g)
-    requires isValidGraph(g')
-    requires g' == removeVertex(g, v)
-    requires optimalValueClique(g, kg)
-    requires optimalValueClique(g', kg')
-    requires kg' == kg
-    requires I <= g.0
-    requires |I| <= kg
-    requires forall i: Node | i in I :: (forall G: Graph | isValidGraph(G) && isSubGraph(G, g) && optimalValueClique(G, kg) :: (forall S: set<Node> | S <= G.0 && optimalClique(G, S) :: i in S));
-    ensures exists S: set<Node> :: S <= g.0 && I<= S && optimalClique(g, S) && v !in S
-{
-    CliqueTranslation(g', kg');
-    assert exists S: set<Node> :: S <= g'.0 && optimalClique(g', S);
-    var S: set<Node> :| S <= g'.0 && isClique(g', S) && |S| == kg' && optimalClique(g', S);
-    CliqueInSubgraph(g, g', kg, S);
-    assert optimalClique(g, S) && v !in S;
 }
