Especificaciones/VertexCover/OptimalCoverPropertiesRemoveVertex.dfy
@@ -1,0 +1,719 @@
+include "VertexCoverOpt.dfy"
+
+//An optimal vertex cover is vertex cover 
+//and its cardinal is the optimal value
+lemma optimalVertexCoverisVertexCover(graph: Graph, I : set<Node>)
+requires isValidGraph(graph) 
+requires optimalVertexCover(graph,I)
+ensures isVertexCover(I,graph)
+ensures optimalValueVertexCover(graph,|I|)
+{}
+
+//|I * {v1,v2}| > 0 is the same as v1 in I || v2 in I
+lemma isVertexCoverEquiv(I:set<Node>, graph:Graph, v1: Node, v2 :Node)
+requires isValidGraph(graph) 
+requires I <= graph.0 && isVertexCover(I,graph)
+requires v1 in graph.0 && v2 in graph.0 && {v1,v2} in graph.1
+ensures v1 in I || v2 in I
+{}
+
+
+lemma biggerOptimalVertexCover(graph : Graph, k : nat, k':nat)
+requires isValidGraph(graph) 
+requires optimalValueVertexCover(graph,k)
+requires  VertexCover(graph, k') && k' <= |graph.0|
+ensures k' >= k
+{}
+
+//The optimal value vertex cover of a subgraph is smaller than that of the graph
+lemma containedOptimalVertexCover(graph : Graph, graph' : Graph, k : nat, k': nat)
+requires isValidGraph(graph) && isValidGraph(graph')
+requires graph'.0 <= graph.0
+requires graph'.1 <= graph.1 
+requires optimalValueVertexCover(graph,k)   
+requires optimalValueVertexCover(graph',k')
+ensures k' <= k
+{
+  var S :| S <= graph.0 && isVertexCover(S, graph) && |S| <= k;
+  var S' := S * graph'.0;
+
+  cardinalityLemma3(S',S);
+  assert |S'| <= |S| <= k;
+  cardinalityLemma3(S',graph'.0);
+  assert |S'| <= |graph'.0|;
+
+  assert isVertexCover(S',graph');
+  biggerOptimalVertexCover(graph',k',|S'|);
+  assert k >= |S'| >= k';
+}
+
+
+
+//A vertex cover whose cardinal is optimal value vertex cover is an optimal vertex cover
+lemma boundVertexCoverIsOptimal(graph : Graph, I : set<Node>, k :nat) 
+requires isValidGraph(graph)
+requires I <= graph.0
+requires isVertexCover(I,graph)
+requires optimalValueVertexCover(graph,k)
+requires |I| <= k
+ensures optimalVertexCover(graph,I)
+{
+ if (!optimalVertexCover(graph,I))
+ {  
+   assert exists S :: S <= graph.0 && isVertexCover(S, graph) && |S| < |I|;
+   var S :| S <= graph.0 && isVertexCover(S, graph) && |S| < |I|;
+   boundoptimalValueVertexCover(graph,k);
+   assert |S| < |I| <= k <= |graph.0|;
+   assert VertexCover(graph,|S|);
+   assert !optimalValueVertexCover(graph,k);
+   assert false;
+ }
+}
+
+//If there are no edges optimal value vertex cover is zero
+lemma OptimalVertexCoverNoEdges(graph : Graph)
+requires isValidGraph(graph)
+requires graph.1 == {}
+ensures optimalValueVertexCover(graph,0)
+{
+   var I : set<Node> := {};
+   assert isVertexCover(I,graph);
+}  
+
+//An edge of fullgraph whose extremes v1, v2 belong to graph'.0 must be in graph'.1
+//because graph is disjoint from I and v1 != v and v2 != v
+lemma subgraphEdges(
+  fullgraph : Graph,
+  I: set<Node>, v : Node,
+  graph : Graph, 
+  graph' : Graph,
+  v1: Node, v2: Node)
+requires isValidGraph(fullgraph) && isValidGraph(graph)  && isValidGraph(graph')
+requires graph.1 +  (set edge:Edge, node:Node | edge in fullgraph.1 && node in I && node in edge :: edge) == fullgraph.1
+requires v in graph.0
+requires I <= fullgraph.0
+requires I * graph.0 == {} && I + graph.0 == fullgraph.0
+requires graph'.0 == graph.0 - { v }
+requires graph'.1 == graph.1 - incidentEdges(graph,v) && {v1,v2} in fullgraph.1
+requires v1 in graph'.0 && v2 in graph'.0
+requires v1 != v && v2 != v && v1 !in I && v2 !in I
+ensures {v1,v2} in graph'.1
+{}
+
+//Moved this lemma to the file Graph.dfy in the folder Especificaciones/Auxiliar
+/*
+lemma validSubgraph(graph : Graph,v : Node, graph': Graph)
+requires isValidGraph(graph)
+requires graph'.0 == graph.0 - { v }
+requires graph'.1 == graph.1 - incidentEdges(graph,v)
+ensures isValidGraph(graph')
+{}
+*/
+
+lemma delVertexCoverCase1(graph : Graph,v : Node, k : nat, graph' : Graph, k' : nat, S':set<Node>)
+requires isValidGraph(graph)  && isValidGraph(graph')
+requires v in graph.0
+requires optimalValueVertexCover(graph,k)   
+requires optimalValueVertexCover(graph',k')
+requires graph'.0 == graph.0 - { v }
+requires graph'.1 == graph.1 - incidentEdges(graph,v)
+requires S' <= graph'.0 && optimalVertexCover(graph', S') && |S'| == k'
+requires forall u:Node | {u,v} in graph.1 :: u in S'
+ensures k' == k
+{ containedOptimalVertexCover(graph,graph',k,k');
+  assert k' <= k;
+
+  assert isVertexCover(S',graph) by{
+       forall e | e in graph.1 
+       ensures |S' * e| > 0
+      { 
+        if (e !in incidentEdges(graph,v)){ }
+        else { 
+          assert e in incidentEdges(graph,v);
+          assert exists u :: u in graph.0 && e == {u,v} && e in incidentEdges(graph,v);
+          var u :| e == {u,v};
+          assert S' * e == {u};
+          assert |S'* e| == 1 > 0;}
+      }
+    }
+        
+
+    assert |S'| == k' <= k;
+    boundVertexCoverIsOptimal(graph,S',k);
+    assert optimalVertexCover(graph,S');
+    assert optimalValueVertexCover(graph,k');
+    assert k == k';
+}
+
+
+lemma delVertexCoverCase2(graph : Graph,v : Node, k : nat, graph' : Graph, k' : nat, S':set<Node>)
+requires isValidGraph(graph)  && isValidGraph(graph')
+requires v in graph.0
+requires optimalValueVertexCover(graph,k)   
+requires optimalValueVertexCover(graph',k')
+requires graph'.0 == graph.0 - { v }
+requires graph'.1 == graph.1 - incidentEdges(graph,v)
+requires S' <= graph'.0 && optimalVertexCover(graph', S') && |S'| == k'
+requires exists u:Node | {u,v} in graph.1 :: u !in S'
+ensures k == k' || k' + 1 == k
+//Not necessarily k == k' + 1
+//Example: v=1, edges (1,2) (2,3)
+//Optimal vertex cover for graph' and graph is both 1 
+{  containedOptimalVertexCover(graph,graph',k,k');
+  assert k' <= k;
+
+  var S := S' + {v};
+  assert |S| == |S'| + 1 == k' + 1;
+
+  assert isVertexCover(S,graph) by{
+       forall e | e in graph.1 
+       ensures |S * e| > 0
+      {
+        if (e !in incidentEdges(graph,v)){}
+        else { 
+          assert v in S * e;
+          assert |S * e| > 0;}
+      }
+      
+    }
+    translationVertexCover(graph,k);
+    var I :| I <= graph.0 && optimalVertexCover(graph, I) && |I| == k;
+    //assert k' + 1 >= k;
+    assert k == k' || k == k' + 1;
+
+}
+
+
+//If we remove a vertex and its incident edges
+//then the optimal value vertex cover may maintain 
+//or be one less
+lemma delVertexCover(graph : Graph,v : Node, k : nat, graph' : Graph, k' : nat)
+requires isValidGraph(graph)  && isValidGraph(graph')
+requires v in graph.0
+requires optimalValueVertexCover(graph,k)   
+requires optimalValueVertexCover(graph',k')
+requires graph'.0 == graph.0 - { v }
+requires graph'.1 == graph.1 - incidentEdges(graph,v)
+ensures k == k' || k == k' + 1
+{ 
+  translationVertexCover(graph',k');
+  var S' :| S' <= graph'.0 && optimalVertexCover(graph', S') && |S'| == k';
+  assert v !in graph'.0 && v !in S';
+  var S := S' + {v};
+  assert |S| == |S'| + 1 == k' + 1;
+  
+  //CASE1 :: all the incident edges are already covered by S', 
+  //so S' is also vertex cover for graph
+  if (forall u:Node | {u,v} in graph.1 :: u in S')
+  { 
+    delVertexCoverCase1(graph,v,k,graph',k',S');
+  }
+  else //CASE2: some incident edge is not covered by S' 
+       //so we add v in order to obtain a vertex cover for graph
+  { 
+    delVertexCoverCase2(graph,v,k,graph',k',S');
+  }
+}
+
+lemma setOfIncidentEdges(graph : Graph,I : set<Node>)
+requires isValidGraph(graph)
+requires I <= graph.0
+requires graph.1 == (set edge:Edge, node:Node | edge in graph.1 && node in I && node in edge :: edge)
+ensures isVertexCover(I,graph)
+{
+}
+
+
+lemma compoundVertexCover(
+  fullgraph : Graph, O : set<Node>, ok: nat, 
+  I: set<Node>, 
+  graph : Graph, k : nat
+)
+requires isValidGraph(fullgraph) && isValidGraph(graph)
+requires graph.0 <= fullgraph.0 && graph.1 <= fullgraph.1 
+requires graph.1 +  (set edge:Edge, node:Node | edge in fullgraph.1 && node in I && node in edge :: edge) == fullgraph.1
+requires I <= fullgraph.0 && I * graph.0 == {} && I + graph.0 == fullgraph.0
+requires optimalValueVertexCover(fullgraph,ok)
+requires optimalValueVertexCover(graph,k)
+requires I <= O <= fullgraph.0 && isVertexCover(O,fullgraph) &&  |O| == ok
+ensures isVertexCover(O-I,graph) && ok == k + |I|
+{
+ translationVertexCover(graph,k);
+ assert |O - I| >= k && ok == |O| == |O - I| + |I| >= k + |I|;
+ 
+  assert ok <= k + |I| by{
+ 
+     var U :| U <= graph.0 && isVertexCover(U,graph) && |U| == k;
+     assert U * I == {};
+     var U' := U + I;
+ 
+     assert U' <= fullgraph.0;
+     forall v1, v2 | {v1,v2} in fullgraph.1 
+     ensures v1 in  U' || v2 in U'
+     ensures |U' * {v1,v2}| > 0
+     {
+       if v1 !in I && v2 !in I
+       { assert {v1,v2} in graph.1;
+         assert v1 in U || v2 in U;
+         assert v1 in U' || v2 in U';
+       }
+       else { assert v1 in I || v2 in I;}
+      }
+     assert isVertexCover(U',fullgraph);
+     assert |U'| == |U| + |I| == k + |I|;
+     translationVertexCover(fullgraph,ok);
+  }
+}
+
+
+
+//In case k == k', there is no optimal vertex cover containing I and v
+
+lemma donotIncludeVertexCoverFull(
+  fullgraph : Graph, O : set<Node>, ok: nat, 
+  vertex: set<Node>, I: set<Node>, v : Node,
+  graph : Graph, k : nat, 
+  graph' : Graph, k' : nat)
+requires isValidGraph(fullgraph) && isValidGraph(graph)  && isValidGraph(graph')
+//graph is obtained from fullgraph by removing vertex in I and their edges
+requires graph.0 <= fullgraph.0 && graph.1 <= fullgraph.1 
+requires graph.1 +  (set edge:Edge, node:Node | edge in fullgraph.1 && node in I && node in edge :: edge) == fullgraph.1
+requires I <= fullgraph.0
+//vertex are not processed yet
+requires vertex <= fullgraph.0 && vertex * I == {} && I * graph.0 == {} && I + graph.0 == fullgraph.0
+requires v in graph.0 && v in vertex
+requires optimalValueVertexCover(fullgraph,ok) 
+requires optimalValueVertexCover(graph,k)   
+requires optimalValueVertexCover(graph',k')
+requires graph'.0 == graph.0 - { v }
+requires graph'.1 == graph.1 - incidentEdges(graph,v)
+requires k == k'
+requires I <= O <= fullgraph.0 && isVertexCover(O,fullgraph) && |O| == ok 
+ensures v !in O
+{
+  
+  var O' := O - I;
+  assert ok == |O| == |I| + |O'|;
+  assert |O'| == ok - |I|;
+  assert isVertexCover(O',graph);
+  translationVertexCover(graph,k); //then ok == k + |I|
+   compoundVertexCover(fullgraph,O,ok,I,graph,k);
+  
+
+  if (v in O)
+ {
+  
+
+  assert isVertexCover(O'- {v}, graph');
+  translationVertexCover(graph',k');
+  assert |O' - {v}| == k' - 1;
+  assert false;
+ }
+
+}
+
+
+//In case k == k', there is no optimal vertex cover containing I and v
+
+lemma donotIncludeVertexCoverFullForall(
+  fullgraph : Graph, ok: nat, 
+  vertex: set<Node>, I: set<Node>, v : Node,
+  graph : Graph, k : nat, 
+  graph' : Graph, k' : nat)
+requires isValidGraph(fullgraph) && isValidGraph(graph)  && isValidGraph(graph')
+//graph is obtained from fullgraph by removing vertex in I and their edges
+requires graph.0 <= fullgraph.0 && graph.1 <= fullgraph.1 
+requires graph.1 +  (set edge:Edge, node:Node | edge in fullgraph.1 && node in I && node in edge :: edge) == fullgraph.1
+requires I <= fullgraph.0
+//vertex are not processed yet
+requires vertex <= fullgraph.0 && vertex * I == {} && I * graph.0 == {} && I + graph.0 == fullgraph.0
+requires v in graph.0 && v in vertex
+requires optimalValueVertexCover(fullgraph,ok) 
+requires optimalValueVertexCover(graph,k)   
+requires optimalValueVertexCover(graph',k')
+requires graph'.0 == graph.0 - { v }
+requires graph'.1 == graph.1 - incidentEdges(graph,v)
+requires k == k'
+ensures forall O : set<Node> | I <= O <= fullgraph.0 && isVertexCover(O,fullgraph) && |O| == ok  :: v !in O
+{
+forall O : set<Node> | I <= O <= fullgraph.0 && isVertexCover(O,fullgraph) && |O| == ok 
+ensures v !in O
+{ donotIncludeVertexCoverFull(fullgraph, O, ok, vertex, I, v, graph, k, graph', k');}
+
+}
+
+//Ik k == k' we do not include v and we still can build a cover for the graph with 
+//the rest of non-processed yet vertex
+lemma donotIncludeVertexCoverExists(
+  fullgraph : Graph, ok: nat, 
+  vertex: set<Node>, I: set<Node>, v : Node,
+  graph : Graph, k : nat,
+  graph' : Graph, k' : nat)
+requires isValidGraph(fullgraph) && isValidGraph(graph)  && isValidGraph(graph')
+requires graph.0 <= fullgraph.0 && graph.1 <= fullgraph.1 
+requires graph.1 +  (set edge:Edge, node:Node | edge in fullgraph.1 && node in I && node in edge :: edge) == fullgraph.1
+requires I <= fullgraph.0
+
+requires vertex <= fullgraph.0 && vertex * I == {} && I * graph.0 == {} && I + graph.0 == fullgraph.0
+requires v in graph.0 && v in vertex
+requires optimalValueVertexCover(fullgraph,ok) 
+requires optimalValueVertexCover(graph,k)   
+requires optimalValueVertexCover(graph',k')
+requires graph'.0 == graph.0 - { v }
+requires graph'.1 == graph.1 - incidentEdges(graph,v)
+requires k == k'
+
+requires exists V : set<Node> :: V <= graph.0 && V <= vertex && optimalVertexCover(graph,V) && optimalVertexCover(fullgraph, I + V)
+ensures exists V' :: V' <= graph.0 && V' <= vertex - {v} && optimalVertexCover(graph,V') && optimalVertexCover(fullgraph, I + V')
+{ translationVertexCover(graph,k);
+  var V :| V <= graph.0 && V <= vertex && optimalVertexCover(graph,V) && optimalVertexCover(fullgraph, I + V);
+  if (v !in V) { assert V <= vertex - {v}; }
+  else { 
+    
+    //this is not possible
+    var V' := V - {v};
+    assert isVertexCover(V',graph');
+    assert |V'| == k - 1 < k';
+    translationVertexCover(graph',k');
+    assert !optimalValueVertexCover(graph',k');
+     assert false;
+  }
+}
+
+//If there are edges in graph.1 then vertex must be non-empty as those edges have not been covered yet
+lemma remainingEdgesImpliesNonEmptyVertex(
+  fullgraph : Graph, ok: nat, 
+  vertex: set<Node>, I: set<Node>, 
+  graph : Graph, k : nat 
+)
+requires isValidGraph(fullgraph) && isValidGraph(graph) 
+requires graph.0 <= fullgraph.0 && graph.1 <= fullgraph.1 
+requires graph.1 +  (set edge:Edge, node:Node | edge in fullgraph.1 && node in I && node in edge :: edge) == fullgraph.1
+requires I <= fullgraph.0
+//vertex are not processed yet
+requires vertex <= fullgraph.0 && vertex * I == {} && I * graph.0 == {} && I + graph.0 == fullgraph.0
+requires exists V : set<Node> :: 
+           V <= graph.0 && V <= vertex &&
+           optimalVertexCover(graph,V)
+ensures graph.1 != {} ==> vertex != {}
+{}
+
+
+//If k == k' + 1 there exists some optimal vertex cover containing v 
+lemma includeVertexCover(graph : Graph,v : Node, k : nat, graph' : Graph, k' : nat)
+requires isValidGraph(graph)  && isValidGraph(graph')
+requires v in graph.0
+requires optimalValueVertexCover(graph,k)   
+requires optimalValueVertexCover(graph',k')
+requires graph'.0 == graph.0 - { v }
+requires graph'.1 == graph.1 - incidentEdges(graph,v)
+requires k == k' + 1
+ensures exists S, S' :: S == S' + {v} && optimalVertexCover(graph,S) && optimalVertexCover(graph',S')
+{
+  translationVertexCover(graph',k');
+  var S' :| S' <= graph'.0 && optimalVertexCover(graph',S') && |S'| == k';
+  var S := S' + {v};
+  assert |S| == k' + 1 == k;
+  assert isVertexCover(S,graph);
+  boundVertexCoverIsOptimal(graph,S,k);
+}
+
+
+//If k == k' + 1 we choose v to be part of the vertex cover 
+//As we know that we can build a cover S' for the remaining graph graph' with vertex 
+// from the set of non-processed yet set of vertex
+// I + S' + {v} will be an optimal vertex cover for the full graph
+lemma includeVertexCoverExists(
+  fullgraph : Graph, ok: nat, 
+  vertex: set<Node>, I: set<Node>, v : Node,
+  graph : Graph, k : nat, 
+  graph' : Graph, k' : nat)
+requires isValidGraph(fullgraph) && isValidGraph(graph)  && isValidGraph(graph')
+//graph is obtained from fullgraph by removing vertex in I and their edges
+requires graph.0 <= fullgraph.0 && graph.1 <= fullgraph.1 
+requires graph.1 +  (set edge:Edge, node:Node | edge in fullgraph.1 && node in I && node in edge :: edge) == fullgraph.1
+requires I <= fullgraph.0
+//vertex are not processed yet
+requires vertex <= fullgraph.0 && vertex * I == {} && I * graph.0 == {} && I + graph.0 == fullgraph.0
+requires v in graph.0 && v in vertex
+requires optimalValueVertexCover(fullgraph,ok) 
+requires optimalValueVertexCover(graph,k)   
+requires optimalValueVertexCover(graph',k')
+requires graph'.0 == graph.0 - { v }
+requires graph'.1 == graph.1 - incidentEdges(graph,v)
+requires k == k' + 1
+requires forall u, O | u in graph.0 && u !in vertex &&  I <= O <= fullgraph.0 && isVertexCover(O,fullgraph) && |O| == ok :: u !in O//optimalVertexCover(fullgraph,O):: u !in O//
+requires exists S ::  S <= graph.0 && S <= vertex && optimalVertexCover(graph,S) && optimalVertexCover(fullgraph, I + S)
+ensures exists S' ::  S' <= graph'.0 && S' <= vertex - {v} && optimalVertexCover(graph',S') && optimalVertexCover(graph, S' + {v}) && optimalVertexCover(fullgraph, I + {v} + S')
+{
+// The size of the optimal vertex cover containing I should be |I| + k
+ assert ok == |I| + k by{
+  var S :| S <= graph.0 && S <= vertex && optimalVertexCover(graph,S) && optimalVertexCover(fullgraph, I + S);
+  boundoptimalVertexCover(fullgraph,I + S);
+  boundoptimalVertexCover(graph,S);
+  assert I * S == {};
+  assert |S| == k && |I + S| == |I| + k == ok;
+ }
+
+ //We know that there exists S' that covers graph' with cardinal k'
+ includeVertexCover(graph,v,k,graph',k');
+ assert exists S, S' :: S == S' + {v} && optimalVertexCover(graph,S) && optimalVertexCover(graph',S');
+ var S' :| S' <= graph'.0 && optimalVertexCover(graph,S' + {v}) && optimalVertexCover(graph',S');
+ optimalVertexCoverisVertexCover(graph',S');
+ assert isVertexCover(S',graph');
+
+ 
+ //lets build O
+ var O := I + {v} + S';
+ 
+ //Check that O is an optimal vertex cover containing I and v
+ assert isVertexCover(O, fullgraph) by
+ {
+  forall v1,v2 | v1 in fullgraph.0 && v2 in fullgraph.0 && {v1,v2} in fullgraph.1
+  ensures v1 in O || v2 in O 
+  ensures |O * {v1,v2}| > 0 
+  {
+   
+    if (v1 == v || v2 == v) {}
+    else if (v1 in I || v2 in I) { }
+    else {
+      assert v1 in graph'.0 && v2 in graph'.0 && S' <= graph'.0 && isVertexCover(S',graph');
+      subgraphEdges(fullgraph,I,v,graph,graph',v1,v2);
+      //assert {v1,v2} in graph'.1;
+      isVertexCoverEquiv(S',graph',v1,v2);
+    }
+  }
+}
+
+//O is optimal because it is vertex cover and it cardinal is ok
+ assert |O| == ok by{
+   calc ==
+   { |O|; 
+    { assert |O| == |I + {v} + S'|;
+      assert (I + {v}) * S' == {};
+    }
+     |I| + 1 + |S'|; 
+     {  boundoptimalVertexCover(graph',S');
+        assert |S'| == k';
+     }
+     |I| + 1 + k' ;  {assert k == k' + 1;}
+     |I| + k;
+     ok;
+   }
+ }
+ boundVertexCoverIsOptimal(fullgraph,O,ok);
+ assert optimalVertexCover(fullgraph, O);
+ 
+ //Vertex in S' should belong to vertex, otherwise they would not belong to an optimal vertex cover
+ forall u | u in S' 
+ ensures u in vertex
+ { assert u in O;
+   if (u !in vertex)
+   {
+    assert I <= O <= fullgraph.0 && optimalVertexCover(fullgraph,O);
+    assert u !in O;
+    assert false;
+
+   }
+ }
+
+
+}
+
+lemma UnionPlusLessElement<T>(A: set<T>, B:set<T>, v:T)
+requires A * B == {}
+requires v !in A && v in B
+ensures (A + {v} ) + (B - {v}) == A + B
+{}
+
+lemma UnionPlusLessSet<T>(A: set<T>, B:set<T>, C:set<T>)
+requires A * B == {}
+requires C <= A  && C * B == {}
+ensures (A - C ) + (B + C) == A + B
+{}
+
+lemma includeVertexAndEdgesProperty(
+  fullgraph : Graph, 
+  I: set<Node>, v : Node,
+  graph : Graph, graph' : Graph)
+requires isValidGraph(fullgraph) && isValidGraph(graph)  && isValidGraph(graph')
+//graph is obtained from fullgraph by removing vertex in I and their edges
+requires graph.0 <= fullgraph.0 && graph.1 <= fullgraph.1 
+requires graph.1 +  (set edge:Edge, node:Node | edge in fullgraph.1 && node in I && node in edge :: edge) == fullgraph.1
+requires I <= fullgraph.0
+requires v in graph.0 && v !in I
+requires I * graph.0 == {}
+requires I + graph.0 == fullgraph.0
+requires graph'.0 == graph.0 - { v }
+requires graph'.1 == graph.1 - incidentEdges(graph,v)
+ensures graph'.1 +  (set edge:Edge, node:Node | edge in fullgraph.1 && node in I + {v} && node in edge :: edge) == fullgraph.1
+ensures (I + {v}) + graph'.0 == fullgraph.0
+{
+  calc == 
+      { (I + {v}) + graph'.0;
+        (I + {v}) + (graph.0 - {v}); 
+        {assert v !in I && v in graph.0; 
+         UnionPlusLessElement(I,graph.0,v);
+        }
+        I + graph.0;
+        fullgraph.0;
+      }
+  var edgesI :=(set edge:Edge, node:Node | edge in fullgraph.1 && node in I && node in edge :: edge);
+  var incidentv := incidentEdges(graph,v);
+  var edgesIv := (set edge:Edge, node:Node | edge in fullgraph.1 && node in I + {v} && node in edge :: edge);
+  calc ==
+  { fullgraph.1;
+    graph.1 +  edgesI;
+    {UnionPlusLessSet(graph.1,edgesI,incidentv);}
+    (graph.1 - incidentv) + (edgesI + incidentv);
+    graph'.1 + (edgesI + incidentv);
+    { assert edgesI + incidentv == edgesIv;}
+    graph'.1 + edgesIv;
+
+
+  }
+}
+
+
+/* Some lemmas that could be useful but that I do not use now:
+
+//Not used
+//Optimal value vertex cover is unique
+lemma oneoptimalValueVertexCover(graph : Graph, k : nat, k': nat)
+requires isValidGraph(graph)
+requires optimalValueVertexCover(graph,k)   
+requires optimalValueVertexCover(graph,k')
+ensures k == k'
+{ assert VertexCover(graph,k);
+  assert VertexCover(graph,k');
+  boundoptimalValueVertexCover(graph,k);
+  boundoptimalValueVertexCover(graph,k');  
+  assert k <= |graph.0| && k' <= |graph.0|;
+  assert k >= k' && k' <= k;
+
+}
+
+
+
+//Not used
+//If the optimal value vertex cover is zero then there are no edges
+lemma zeroOptimalVertexCover(graph : Graph)
+requires isValidGraph(graph)
+requires optimalValueVertexCover(graph,0)
+ensures graph.1 == {}
+{
+    if graph.1 != {} 
+    {
+        var e :| e in graph.1;
+        var I : set<Node> :| |I| == 0 && isVertexCover(I,graph);
+        assert I == {} && |I * e| == 0;
+        assert false;
+    }
+}  
+
+
+//Not used
+lemma emptyIncidentEdges(graph : Graph, v : Node)
+requires isValidGraph(graph)
+requires v in graph.0
+requires incidentEdges(graph,v) == {}
+ensures forall e | e in graph.1 :: v !in e
+{
+  forall e | e in graph.1
+  ensures v !in e
+  { if (v in e) {
+    assert e in incidentEdges(graph,v);
+    assert false;
+  }
+  }
+
+}
+
+//Not used
+lemma nonEmptyIncidentEdges(graph : Graph, v : Node)
+requires isValidGraph(graph)
+requires v in graph.0
+requires incidentEdges(graph,v) != {}
+ensures exists u:Node :: u in graph.0 && {u,v} in graph.1
+{
+  var e :| e in incidentEdges(graph,v);
+  assert exists u :: u in graph.0 && {u,v} == e;
+}
+
+//Not used
+//If a vertex has no incident edges 
+//then it does not belong to any optimal vertex cover
+lemma  OptimalVertexCoverAlone(graph : Graph, I: set<Node>, v : Node)
+requires isValidGraph(graph)
+requires v in graph.0
+requires incidentEdges(graph,v) == {}
+requires optimalVertexCover(graph,I)
+ensures v !in I
+{
+  if (v in I)
+  {
+   var I' := I - {v};
+   emptyIncidentEdges(graph,v);
+   assert isVertexCover(I',graph);
+   assert false;
+  }
+}
+
+//Not used
+//If we remove a vertex without incident edges
+//the optimal value vertex cover does not change
+lemma OptimalVertexCoverNoIncidentEdges(graph : Graph, v : Node, k : nat, graph' : Graph)
+requires isValidGraph(graph)
+requires v in graph.0
+requires incidentEdges(graph,v) == {}
+requires graph'.0 == graph.0 - { v }
+requires graph'.1 == graph.1 - incidentEdges(graph,v)
+requires optimalValueVertexCover(graph,k)
+ensures optimalValueVertexCover(graph',k)
+{
+    var I : set<Node> :| I <= graph.0 && |I| <= k 
+                         && isVertexCover(I,graph);
+    
+    //I is optimal
+    boundVertexCoverIsOptimal(graph,I,k);
+    assert optimalVertexCover(graph,I);
+    // and it does not contain v, so it is also a cover of graph'
+    OptimalVertexCoverAlone(graph,I,v);
+    assert isVertexCover(I,graph');
+    assert VertexCover(graph',k);
+
+    //k is optimal value because it is optimal for graph
+    forall x : nat |  x <= |graph'.0| && VertexCover(graph', x) 
+    ensures x >= k
+    { assert VertexCover(graph, x);
+     
+    }
+}
+
+//Not used
+lemma donotIncludeVertexCover(graph : Graph,v : Node, k : nat, graph' : Graph, k' : nat)
+requires isValidGraph(graph)  && isValidGraph(graph')
+requires v in graph.0
+requires optimalValueVertexCover(graph,k)   
+requires optimalValueVertexCover(graph',k')
+requires graph'.0 == graph.0 - { v }
+requires graph'.1 == graph.1 - incidentEdges(graph,v)
+requires k == k'
+ensures exists S :: v !in S && optimalVertexCover(graph,S) && optimalVertexCover(graph',S)
+{
+  translationVertexCover(graph,k);
+  var S :| S <= graph.0 && optimalVertexCover(graph,S) && |S| == k;
+  if (v !in S)
+    { assert S <= graph'.0;
+      boundVertexCoverIsOptimal(graph',S,k);
+      assert optimalVertexCover(graph',S);
+    } 
+   else { //This is not compatible with k == k'
+      var S' := (S - {v});
+      assert |S'| == k - 1 < k;
+      translationVertexCover(graph',k);
+      assert false;
+    }
+}
+
+*/
