Especificaciones/VertexCover/VertexCoverOpt.dfy
@@ -1,0 +1,64 @@
+include "VertexCover.dfy"
+//predicado de PCV
+ghost predicate optimalValueVertexCover (graph : Graph, k : nat) 
+    requires isValidGraph(graph) 
+{     
+    VertexCover(graph, k) 
+   && forall x : nat |  x <= |graph.0| && VertexCover(graph, x) :: x >= k
+} 
+//In this definition the bound x <= |graph.0| does not constraint anything
+// because VertexCover(graph, |graph.0|) always holds
+//There cannot exist x > |graph.0| such that k > x.
+//Otherwise we have that k > |graph.0|  
+
+
+//Optimal value vertex cover will never be strictly higher than |graph.0|
+//because VertexCover(graph, |graph.0|) always holds
+
+lemma boundoptimalValueVertexCover(graph: Graph, k : nat) 
+requires isValidGraph(graph)
+requires optimalValueVertexCover(graph,k)
+ensures k <= |graph.0|
+{ 
+    assert VertexCover(graph,|graph.0|);
+}
+
+lemma emptyOptimalValueVertexCover(graph: Graph) 
+requires isValidGraph(graph)
+ensures graph.1 == {} ==> optimalValueVertexCover(graph, 0)
+{
+    assert graph.1 == {} ==> isVertexCover({}, graph);
+}
+
+//POCV predicate 
+//S to denote sets
+ghost predicate optimalVertexCover (graph: Graph, I : set<Node>)
+    requires isValidGraph(graph) 
+{
+       I <= graph.0 
+    && isVertexCover(I, graph) 
+    && forall S: set<Node> | S <= graph.0 && isVertexCover(S, graph) :: |S| >= |I|
+}
+
+
+lemma boundoptimalVertexCover(graph: Graph, I : set<Node>) 
+requires isValidGraph(graph)
+requires optimalVertexCover(graph,I)
+ensures |I| <= |graph.0|
+ensures optimalValueVertexCover(graph,|I|)
+{  }
+
+lemma translationVertexCover(graph: Graph, k: nat) 
+requires isValidGraph(graph)
+requires optimalValueVertexCover(graph, k)
+ensures exists I: set<Node> :: I <= graph.0 && optimalVertexCover(graph, I) && |I| == k
+ensures !exists I:set<Node> | I <= graph.0 && |I| < k  :: isVertexCover(I,graph)
+{
+    if exists I:set<Node> :: I <= graph.0 && |I| < k && isVertexCover(I,graph)
+    {
+        ghost var I: set<Node> :| I <= graph.0 && |I| < k && isVertexCover(I,graph);
+        assert VertexCover(graph, |I|);
+        cardinalityLemma3(I, graph.0);
+        assert false;
+    }
+}
