Turing Reducciones/Clique/POCToPCAux.dfy
@@ -1,0 +1,130 @@
+include "../../Especificaciones/Clique/CliqueOpt.dfy"
+include "../../Especificaciones/Clique/CliqueProperties.dfy"
+
+lemma ovCliqueRemoveVertex(g: Graph, g': Graph, v: Node, kg: nat, kg': nat)
+    requires isValidGraph(g)
+    requires g' == removeVertex(g, v)
+    requires isSubGraph(g', g)
+    requires optimalValueClique(g, kg)
+    requires optimalValueClique(g', kg')
+    ensures kg' == kg || kg == kg' + 1
+{
+    if kg' > kg {
+        ghost var I: set<Node> :| I <= g'.0 && isClique(g', I) && |I| >= kg';
+        assert CliqueDecissionProblem(g, |I|);
+        assert false;
+    }
+    assert kg >= kg';
+    CliqueTranslation(g, kg);
+    //No entiendo por qué no es capaz de sacar cosas que están en la definición de optimalClique
+    ghost var I: set<Node> :| (optimalClique(g, I) && |I| == kg && I <= g.0 && isClique(g, I));
+    assert isClique(g, I);
+    assert v in I || v !in I;
+    if v !in I {
+        assert optimalValueClique(g', |I|);
+    }
+    else{
+        if exists I': set<Node> :: isClique(g', I') && |I'| == kg {}
+        else{
+            ghost var I': set<Node> := I - {v};
+            CliqueTranslation2(g', I');
+        }
+    } 
+}
+
+lemma isPartialSolutionWith1(g: Graph, g': Graph, v: Node, kg: nat, kg': nat)
+    requires isValidGraph(g)
+    requires isValidGraph(g')
+    requires g' == removeVertex(g, v)
+    //requires isSubGraph(g', g)
+    requires optimalValueClique(g, kg)
+    requires optimalValueClique(g', kg')
+    requires kg' < kg
+    ensures forall S: set<Node> | S <= g.0 && optimalClique(g, S) :: v in S
+{
+    //all optimal cliques in g must contain v
+    assert (forall A: set<Node> | optimalClique(g, A) :: v in A) by {
+        if exists A: set<Node> :: optimalClique(g, A) && v !in A
+        {
+            var A: set<Node> :| optimalClique(g, A) && v !in A;
+            assert isClique(g', A);
+            assert optimalValueClique(g', |A|);
+            assert |A| > kg';
+            assert false;
+        }
+    }
+}
+
+lemma isPartialSolutionWith2(g: Graph, g': Graph, v: Node, kg: nat, kg': nat)
+    requires isValidGraph(g)
+    requires isValidGraph(g')
+    requires g' == removeVertex(g, v)
+    requires optimalValueClique(g, kg)
+    requires optimalValueClique(g', kg')
+    requires kg' + 1 == kg
+    ensures forall G: Graph | isValidGraph(G) && isSubGraph(G, g) && optimalValueClique(G, kg) :: (forall S: set<Node> | S <= G.0 && optimalClique(G, S) :: v in S)
+{
+    //if there exists a subgraph whose optimal clique does not include v
+    if exists G: Graph :: isValidGraph(G) && isSubGraph(G, g) && optimalValueClique(G, kg) && (exists S: set<Node> :: S <= G.0 && optimalClique(G, S) && v !in S)
+    {
+        //instantiate the graph
+        var G: Graph :| isValidGraph(G) && isSubGraph(G, g) && optimalValueClique(G, kg) && (exists S: set<Node> :: S <= G.0 && optimalClique(G, S) && v !in S);
+        //instantiate the clique
+        var S: set<Node> :| S <= G.0 && optimalClique(G, S) && v !in S; 
+        //that clique must actually contain v, since it would be an optimal clique in g
+        CliqueTranslation2(G, S);
+        assert |S| == kg;
+        CliqueInSubgraph(g, G, |S|, S);
+        assert optimalClique(g, S);
+        isPartialSolutionWith1(g, g', v, kg, kg');
+    }
+}
+
+lemma isPartialSolutionWith(g: Graph, g': Graph, v: Node, kg: nat, kg': nat, I: set<Node>)
+    decreases I
+    requires isValidGraph(g)
+    requires isValidGraph(g')
+    requires g' == removeVertex(g, v)
+    requires optimalValueClique(g, kg)
+    requires optimalValueClique(g', kg')
+    requires kg' + 1 == kg
+    requires I <= g.0
+    requires |I| <= kg
+    requires forall i: Node | i in I :: (forall G: Graph | isValidGraph(G) && isSubGraph(G, g) && optimalValueClique(G, kg) :: (forall S: set<Node> | S <= G.0 && optimalClique(G, S) :: i in S))
+    ensures exists S: set<Node> :: S <= g.0 && I <= S && optimalClique(g, S) && v in S
+{
+    //all optimal cliques in g must contain v
+    assert (forall A: set<Node> | optimalClique(g, A) :: v in A) by {
+        if exists A: set<Node> :: optimalClique(g, A) && v !in A
+        {
+            var A: set<Node> :| optimalClique(g, A) && v !in A;
+            assert isClique(g', A);
+            assert optimalValueClique(g', |A|);
+            assert |A| > kg';
+            assert false;
+        }
+    }
+    alwaysAnOptimalClique(g);
+    assert exists S: set<Node> :: S <= g.0 && optimalClique(g, S) && v in S;
+    var S: set<Node> :| S <= g.0 && optimalClique(g, S) && v in S; 
+    assert forall i: Node | i in I :: i in S; 
+}
+
+lemma isPartialSolutionWithout(g: Graph, g': Graph, v: Node, kg: nat, kg': nat, I: set<Node>)
+    requires isValidGraph(g)
+    requires isValidGraph(g')
+    requires g' == removeVertex(g, v)
+    requires optimalValueClique(g, kg)
+    requires optimalValueClique(g', kg')
+    requires kg' == kg
+    requires I <= g.0
+    requires |I| <= kg
+    requires forall i: Node | i in I :: (forall G: Graph | isValidGraph(G) && isSubGraph(G, g) && optimalValueClique(G, kg) :: (forall S: set<Node> | S <= G.0 && optimalClique(G, S) :: i in S))
+    ensures exists S: set<Node> :: S <= g.0 && I<= S && optimalClique(g, S) && v !in S
+{
+    CliqueTranslation(g', kg');
+    assert exists S: set<Node> :: S <= g'.0 && optimalClique(g', S);
+    var S: set<Node> :| S <= g'.0 && isClique(g', S) && |S| == kg' && optimalClique(g', S);
+    CliqueInSubgraph(g, g', kg, S);
+    assert optimalClique(g, S) && v !in S;
+}
